theories/interop/gctoken.v
@@ -1,0 +1,67 @@
+From Coq Require Import ssreflect.
+From stdpp Require Import strings gmap.
+From melocoton Require Import named_props.
+From iris.base_logic.lib Require Import ghost_map ghost_var.
+From iris.algebra Require Import gset.
+From iris.proofmode Require Import proofmode.
+From melocoton.c_interface Require Import defs resources.
+From melocoton.ml_lang Require Import lang lang_instantiation primitive_laws.
+From melocoton.interop Require Import basics basics_resources.
+
+(* The [GC θ] resource.
+
+   [GC θ] represents the collection of authoritative resources related to the ML
+   runtime while running or interoperating with external C-like code. It is used
+   e.g. in the points-to update laws that translate between ML and block-level
+   pointsto.
+
+   Its definition is best understood side-by-side with the wrapper state
+   interpretation (in weakestpre.v), but is in its own separate file to make it
+   possible to only import [GC θ] and relevant SL resources without depending on
+   the wrapper WP and state interp.
+ *)
+
+Class wrapperGCtokGS Σ := WrapperGCtokGS {
+  wrapperGS_basics :> wrapperBasicsGS Σ;
+  wrapperGS_locsetGS :> ghost_varG Σ (gsetUR loc);
+  wrapperGS_addrmapGS :> ghost_varG Σ (leibnizO addr_map);
+  wrapperGS_var_lstoreGS :> ghost_varG Σ lstore;
+  wrapperGS_var_lloc_mapGS :> ghost_varG Σ lloc_map;
+  wrapperGS_γζ : gname;
+  wrapperGS_γθ : gname;
+  wrapperGS_γχ : gname;
+  wrapperGS_γroots_set : gname;
+}.
+
+Section GCtoken.
+Context {hlc : has_lc}.
+Context {Σ : gFunctors}.
+Context `{!heapGS_ML Σ, !heapGS_C Σ}.
+Context `{!wrapperGCtokGS Σ}.
+
+Definition GC (θ : addr_map) : iProp Σ :=
+  ∃ (ζ ζfreeze ζσ ζvirt : lstore) (χ χvirt : lloc_map) (σMLvirt : store)
+    (roots_s : gset addr) (roots_m : gmap addr lval),
+    "GCζ" ∷ ghost_var wrapperGS_γζ (1/2) ζ
+  ∗ "GCχ" ∷ ghost_var wrapperGS_γχ (1/2) χ
+  ∗ "GCθ" ∷ ghost_var wrapperGS_γθ (1/2) θ
+  ∗ "GCroots" ∷ ghost_var wrapperGS_γroots_set (1/2) roots_s
+  ∗ "GCζvirt" ∷ lstore_own_auth ζvirt
+  ∗ "(GCσMLv & GCσdom)" ∷ state_interp (σMLvirt : language.language.state ML_lang)
+  ∗ "GCχvirt" ∷ lloc_own_auth χvirt
+  ∗ "GCχNone" ∷ ([∗ map] _↦ℓ ∈ pub_locs_in_lstore χvirt ζvirt, ℓ ↦M/)
+  ∗ "GCrootsm" ∷ ghost_map_auth wrapperGS_γroots_map 1 roots_m
+  ∗ "GCrootspto" ∷ ([∗ map] a ↦ v ∈ roots_m, ∃ w, a ↦C w ∗ ⌜repr_lval θ v w⌝)
+  ∗ "%Hrootsdom" ∷ ⌜dom roots_m = roots_s⌝
+  ∗ "%Hrootslive" ∷ ⌜roots_are_live θ roots_m⌝
+  ∗ "%Hfreezeρ" ∷ ⌜freeze_lstore ζ ζfreeze⌝
+  ∗ "%Hfreezeeq" ∷ ⌜ζfreeze = ζσ ∪ ζvirt⌝
+  ∗ "%Hfreezedj" ∷ ⌜ζσ ##ₘ ζvirt⌝
+  ∗ "%Hstore_blocks" ∷ ⌜is_store_blocks χvirt σMLvirt ζσ⌝
+  ∗ "%Hother_blocks" ∷ ⌜dom ζvirt ⊆ dom χvirt⌝
+  ∗ "%Hstore" ∷ ⌜is_store χvirt ζfreeze σMLvirt⌝
+  ∗ "%Hχvirt" ∷ ⌜expose_llocs χ χvirt⌝
+  ∗ "%Hχinj" ∷ ⌜lloc_map_inj χ⌝ (* TODO redundant? *)
+  ∗ "%HGCOK" ∷ ⌜GC_correct ζfreeze θ⌝.
+
+End GCtoken.
