theories/interop/wp_ext_call_laws.v
@@ -10,7 +10,7 @@ From iris.algebra Require Import gset gset_bij.
 From iris.proofmode Require Import proofmode.
 From melocoton.c_interface Require Import defs notation resources.
 From melocoton.ml_lang Require Import lang lang_instantiation primitive_laws.
-From melocoton.interop Require Import basics prims weakestpre wp_block_sim wp_utils.
+From melocoton.interop Require Import basics prims weakestpre wp_utils.
 Import Wrap.
 
 Section Laws.
